draft: allocator toy impl wrt Array model
-> concretize Array model
-> C extraction ?
-> ordering issue: arr wrt asel arr h,
should both of these be equal?

src/Allocator.fst
@@ -1,15 +1,34 @@
 module Allocator
 
-open FStar.List.Tot
+module L = FStar.List.Tot
+open FStar.Ref
+module Seq = FStar.Seq
 open Some_lemmas
 
-let size_header = 0
 
+(*
+let size_header = 0
+noeq
+type t2 =
+| Blah : unit -> t2
+type bytes_ = Seq.seq t2
+let b : FStar.UInt8.byte = FStar.UInt8.zero
+let bs1 : bytes_ = Seq.create 10 (Blah ())
+let bs2 : bytes_ = Seq.create 10 (Blah  ())
+
+[@@ expect_failure]
+let test = bs1 = bs2
+*)
+
+//type bytes (s: nat) = Seq.lseq FStar.UInt8.byte s
+type bytes (s: nat) = Seq.seq FStar.UInt8.byte
+//type bytes = Seq.seq FStar.UInt8.byte
 noeq
 type block = {
   size: nat;
   is_free: bool;
-  content: nat;
+  //content: ref (bytes size);
+  content: bytes size;
 }
 
 type lblock = list block
@@ -27,6 +46,56 @@ let mk_block size is_free content = {
 let is_free (b: block) : bool
   = get_is_free b
 
+let split_block (blk: block) (size: nat)
+  : Pure (block & block)
+  (size <= get_size blk /\
+  get_size blk = Seq.length (get_content blk)
+  )
+  (fun (b1, b2) ->
+    get_size b1 = size /\
+    get_size blk = get_size b1 + get_size b2  /\
+    //not (is_free b1) /\ is_free b2 /\
+    get_content blk = Seq.append (get_content b1) (get_content b2)
+  )
+  =
+  let initial_bytes = get_content blk in
+  let bytes1, bytes2 = Seq.split initial_bytes size in
+  let blk1 = mk_block size true bytes1 in
+  let blk2 = mk_block (get_size blk - size) true bytes2 in
+  Seq.lemma_split initial_bytes size;
+  blk1, blk2
+
+let split_block_lemma (blk: block) (size: nat)
+  : Lemma
+  (requires
+    size <= get_size blk /\
+    get_size blk = Seq.length (get_content blk)
+  )
+  (ensures 
+    (let b1, b2 = split_block blk size in
+    let bytes = get_content b1, get_content b2 in
+    bytes = Seq.split (get_content blk) size))
+  = ()
+
+(*)
+let rec malloc (l: lblock) (size: nat)
+: lblock & option (bytes size)
+= match l with
+| [] ->
+    let status = 1 in
+    [], None
+| x::l' ->
+    let block_size = get_size x in
+    if size <= get_size x
+    then
+      let block1, block2 = split_block x size in
+      let abytes = get_content block1 in
+      block1::block2::l', Some abytes
+    else
+      let lblock, abytes = malloc l' size in
+      x::lblock, abytes
+
+(*)
 let f (x y: block)
   = not (is_free x && is_free y)
 
@@ -70,9 +139,13 @@ let rec coalesce_aux (acc l: lblock)
     if is_free x && is_free y then
       let size_x = get_size x in
       let size_y = get_size y in
-      let new_size = size_x + size_y - size_header in
+      let new_size = size_x + size_y in
+      //- size_header in
       let new_is_free = true in
-      let new_content = 0 in
+      let content_x = get_content x in
+      let content_y = get_content y in
+      let new_content = Seq.append content_x content_y in
+      //write content_x_ref new_content;
       let new_block = mk_block new_size new_is_free new_content in
       coalesce_aux acc (new_block::l')
     else if not (is_free y) then
@@ -109,9 +182,12 @@ let rec coalesce_aux_proof (acc l: lblock)
     if is_free x && is_free y then begin
       let size_x = get_size x in
       let size_y = get_size y in
-      let new_size = size_x + size_y - size_header in
+      let new_size = size_x + size_y in
+      //- size_header in
       let new_is_free = true in
-      let new_content = 0 in
+      let content_x = get_content x in
+      let content_y = get_content y in
+      let new_content = Seq.append content_x content_y in
       let new_block = mk_block new_size new_is_free new_content in
       coalesce_aux_proof acc (new_block::l')
     end else if not (is_free y) then begin
